state end2end_lightbulb, and sketch its proof

end2end/src/End2EndLightbulb.v
@@ -4,7 +4,7 @@ Require Import Coq.Lists.List. Import ListNotations.
 Require Import coqutil.Word.Interface.
 Require Import coqutil.Map.Interface.
 Require Import bedrock2.Syntax.
-Require Import bedrock2.Examples.lightbulb.
+Require Import bedrock2.Examples.lightbulb bedrock2.Examples.lightbulb_spec.
 Require Import bedrock2.TracePredicate. Import TracePredicateNotations.
 Require Import compiler.ProgramSpec.
 Require Import compiler.MemoryLayout.
@@ -27,25 +27,32 @@ Instance mapops: RegAlloc.map.ops (SortedListString.map Z). refine (
 Defined.
 
 Definition instrMemSizeLg: Z := 10. (* TODO is this enough? *)
+Lemma instrMemSizeLg_bounds : 3 <= instrMemSizeLg <= 30. Proof. cbv. intuition discriminate. Qed.
 Definition dataMemSize: Z := 4096.
 
-Definition funnamesList: list string.
+Definition FunctionImpl: Type :=
+  (list string * list string * @cmd (StringNamesSyntax.make BasicCSyntax.StringNames_params)).
+
+Definition funimplsList: list (string * FunctionImpl).
   match type of link_lightbulb with
-  | spec_of_iot ?L => let r := eval cbv in (List.map fst L) in exact r
+  | spec_of_iot ?L => exact L
   end.
 Defined.
 
+Definition funnamesList: list string := Eval cbv in List.map fst funimplsList.
+Definition funimplsListWithoutNames: list FunctionImpl := Eval cbv in List.map snd funimplsList.
+
 Definition funimplsMap: Semantics.env.
-  match type of link_lightbulb with
-  | spec_of_iot ?L =>
-    let keys := eval cbv in (List.map fst L) in
-    let values := eval cbv in (List.map snd L) in
-    let o := eval cbv in (@map.of_list _ _ Semantics.env keys values) in
-    lazymatch o with
-    | Some ?m => exact m
-    end
+  let o := eval cbv in (@map.of_list _ _ Semantics.env funnamesList funimplsListWithoutNames) in
+  lazymatch o with
+  | Some ?m => exact m
   end.
 Defined.
+
+Definition funspecs: funname ->
+   Semantics.trace -> Semantics.mem -> list Semantics.word ->
+   (Semantics.trace -> Semantics.mem -> list Semantics.word -> Prop) -> Prop
+  := WeakestPrecondition.call funimplsList.
 
 Definition buffer_addr: Z. Admitted.
 
@@ -59,8 +66,17 @@ Definition prog := {|
   loop_body := @cmd.call Semantics.syntax ["res"] "iot" [expr.literal buffer_addr];
 |}.
 
+Definition lightbulb_packet_rep: bool -> list Semantics.byte -> Prop.
+  intros command bytes.
+  refine (lightbulb_packet_rep command (_ bytes)).
+  case TODO.
+Defined.
+
 Definition traceOfOneInteraction: list (lightbulb_spec.OP Semantics.word) -> Prop :=
-  (existsl (fun bytes => lightbulb_spec.lan9250_recv _ _ bytes)) |||
+  (fun t => exists packet cmd, (lan9250_recv _ _ packet +++ gpio_set _ 23 cmd) t /\
+                               lightbulb_packet_rep cmd packet) |||
+  (fun t => exists packet, lan9250_recv _ _ packet t /\
+                           ~ (exists cmd : bool, lightbulb_packet_rep cmd packet)) |||
   (lightbulb_spec.lan9250_recv_no_packet _ _) |||
   (lightbulb_spec.lan9250_recv_packet_too_long _ _) |||
   (any +++ (lightbulb_spec.spi_timeout _)).
@@ -82,7 +98,7 @@ Definition spec: ProgramSpec := {|
                                goodHlTrace ioh;
   isReady t m l := exists buf R,
     (Separation.sep (Array.array Scalars.scalar8 (word.of_Z 1) (word.of_Z buffer_addr) buf) R) m /\
-    length buf = 1520%nat;
+    Z.of_nat (Datatypes.length buf) = 1520;
 |}.
 
 Definition ml: MemoryLayout 32. Admitted.
@@ -99,11 +115,84 @@ Lemma instrMemSizeLg_agrees_with_ml:
   word.sub (code_pastend ml) (code_start ml) = word.of_Z instrMemSizeLg.
 Admitted.
 
-Lemma end2end_lightbulb: False.
+Lemma link_lightbulb_withCorrectWordInstance:
+  forall (p_addr : Semantics.word) (buf : list Semantics.byte) (R : Semantics.mem -> Prop)
+         (m : Semantics.mem) (t : Semantics.trace),
+    Separation.sep (Array.array Separation.ptsto (word.of_Z 1) p_addr buf) R m ->
+    Z.of_nat (Datatypes.length buf) = 1520 ->
+    WeakestPrecondition.call
+      [iot; recvEthernet; lightbulb; LAN9250.lan9250_readword; SPI.spi_xchg; SPI.spi_read;
+         SPI.spi_write] "iot" t m [p_addr]
+      (fun (t' : Semantics.trace) (_ : Semantics.mem) (rets : list Semantics.word) =>
+         exists v : Semantics.word,
+           rets = [v] /\
+           (exists iol,
+               t' = (iol ++ t)%list /\
+               (exists ioh,
+                   relate_lightbulb_trace_to_bedrock ioh iol /\
+                   ((exists packet (cmd : bool),
+                        (lan9250_recv _ _ packet +++ gpio_set Semantics.word 23 cmd) ioh /\
+                        lightbulb_packet_rep cmd packet /\ word.unsigned v = 0) \/
+                    (exists packet : list Semantics.byte,
+                        lan9250_recv _ _ packet ioh /\
+                        ~ (exists cmd : bool, lightbulb_packet_rep cmd packet) /\
+                        word.unsigned v = 0) \/
+                    (lan9250_recv_no_packet _ _ ioh /\ word.unsigned v = 0) \/
+                    (lan9250_recv_packet_too_long _ _ ioh /\ word.unsigned v <> 0) \/
+                    ((any +++ spi_timeout Semantics.word) ioh /\ word.unsigned v <> 0))))).
 Proof.
-  pose proof link_lightbulb as P.
-  unfold spec_of_iot in *.
+  replace semantics with FE310CSemantics.parameters. (* silently fails *) Undo.
+  Fail pattern semantics.
+  pose proof link_lightbulb as P. unfold spec_of_iot in P.
+  (* TODO andres why is there no separation logic assertion in the postcondition? *)
+  Fail apply P.
+  case TODO.
+Qed.
 
+Lemma weaken_call: forall funs fname t m args (post1 post2: _ -> _ -> _ -> Prop),
+    WeakestPrecondition.call funs fname t m args post1 ->
+    (forall t' m' l', post1 t' m' l' -> post2 t' m' l') ->
+    WeakestPrecondition.call funs fname t m args post2.
+Proof.
+  intros.
+Admitted.
+
+Lemma relate_concat: forall ioh1 ioh2 iol1 iol2,
+    relate_lightbulb_trace_to_bedrock ioh1 iol1 ->
+    relate_lightbulb_trace_to_bedrock ioh2 iol2 ->
+    relate_lightbulb_trace_to_bedrock (ioh2 ++ ioh1) (iol2 ++ iol1)%list.
+Admitted.
+
+Lemma relate_nil: relate_lightbulb_trace_to_bedrock [] [].
+Admitted.
+
+Lemma goodHlTrace_addOne: forall iohNew ioh,
+    traceOfOneInteraction iohNew ->
+    goodHlTrace ioh ->
+    goodHlTrace (iohNew ++ ioh).
+Proof.
+  intros. unfold goodHlTrace. apply kleene_app.
+  - change iohNew with ([] ++ iohNew)%list.
+    apply kleene_step. 1: assumption. apply kleene_empty.
+  - assumption.
+Qed.
+
+Ltac destr :=
+  repeat match goal with
+         | A: exists x, _ |- _ => let x' := fresh x in destruct A as [x' ?]
+         | A: _ /\ _ |- _ => destruct A as [? ?]
+         end.
+
+Lemma end2end_lightbulb: forall (t: Semantics.LabelSeqT) (mFinal: KamiRiscv.KamiImplMachine),
+    Semantics.Behavior (p4mm instrMemSizeLg instrMemSizeLg_bounds) mFinal t ->
+    exists t': list KamiRiscv.Event,
+      KamiRiscv.KamiLabelSeqR t t' /\
+      (exists (suffix : list KamiRiscv.Event) (bedrockTrace : list RiscvMachine.LogItem),
+          KamiRiscv.traces_related (suffix ++ t') bedrockTrace /\
+          (exists ioh : list (lightbulb_spec.OP _),
+              relate_lightbulb_trace_to_bedrock ioh bedrockTrace /\ goodHlTrace ioh)).
+Proof.
+  (* Fail eapply @end2end. unification only works after some specialization *)
   pose proof @end2end as Q.
   specialize_first Q mapops.
   specialize_first Q prog.
@@ -111,5 +200,41 @@ Proof.
   specialize_first Q spec.
   specialize_first Q mlOk.
   specialize_first Q memInit.
+  specialize_first Q funspecs.
 
-Abort.
+  unfold bedrock2Inv, goodTraceE, isReady, goodTrace, spec in *.
+  eapply Q; clear Q; cycle 1.
+  - (* preserve invariant *)
+    intros.
+    (* TODO make Simp.simp work here *)
+    destruct H as [ [ buf [R [Sep L] ] ] [ioh [Rel G] ] ].
+    pose proof link_lightbulb_withCorrectWordInstance as P.
+    unfold spec_of_iot in *.
+    specialize_first P Sep.
+    specialize_first P L.
+    cbv [loop_body funspecs funimplsList prog
+         WeakestPrecondition.cmd WeakestPrecondition.cmd_body].
+    eexists. split; [reflexivity|].
+    eapply weaken_call; [eapply P|clear P].
+    cbv beta.
+    intros.
+    destr.
+    subst.
+    eexists. split; [reflexivity|].
+    split.
+    + case TODO. (* iot should preserve what it requires as a precondition *)
+    + destruct H2 as [ C | [C | [C | [C | C ] ] ] ];
+        destr; eexists (ioh0 ++ ioh)%list; (split;
+        [ eapply relate_concat; assumption
+        | apply goodHlTrace_addOne;
+          [unfold traceOfOneInteraction, choice; eauto 10
+          | exact G]]).
+  - (* establish invariant *)
+    intros.
+    unfold init_code, prog.
+    hnf. split.
+    + case TODO. (* how can we relate m to Kami's mem and constrain it? *)
+    + exists []. split.
+      * apply relate_nil.
+      * unfold goodHlTrace. apply kleene_empty.
+Qed. (* takes more than 30s *)
